Lentil reloaded

Lentil/Basic.lean
@@ -1,85 +1,238 @@
-import Aesop
-import Mathlib.Data.List.Basic
-import Mathlib.Tactic.Linarith
-import Mathlib.Tactic.PushNeg
-import Duper
+import Lean
+import Batteries.Util.ExtendedBinder
 
--- basic semantics & connectives
+open Lean
 
-def exec (α : Type) := ℕ → α
-def predicate (α : Type) := exec α → Prop
+-- a small library about TLA, with only currently required things
 
-def state_pred {α : Type} (f : α → Prop) : predicate α :=
-  λ σ ↦ f (σ 0)
+namespace TLA
 
-notation:50 "⌜" p "⌝" => (state_pred p)
+-- this part is from `TransitionSystem`; any better way for inheriting those definitions?
+def exec (σ : Type) := Nat → σ
+def pred (σ : Type) := exec σ → Prop
+def state_pred {σ : Type} (f : σ → Prop) : pred σ :=
+  fun e => f (e 0)
+def action (σ : Type) := σ → σ → Prop
+def action_pred {σ : Type} (a : action σ) : pred σ :=
+  fun e => a (e 0) (e 1)
 
-def pure_pred {α : Type} (p : Prop) : predicate α := ⌜ λ _ ↦ p ⌝
+def pure_pred {α : Type} (p : Prop) : pred α := state_pred (fun _ => p)
+def tla_true {α : Type} : pred α := pure_pred True
+def tla_false {α : Type} : pred α := pure_pred False
 
-notation:50 "⌞" p "⌟" => (pure_pred p)
+def tla_and {α : Type} (p q : pred α) : pred α := fun σ => p σ ∧ q σ
+def tla_or {α : Type} (p q : pred α) : pred α := fun σ => p σ ∨ q σ
+def tla_implies {α : Type} (p q : pred α) : pred α := fun σ => p σ → q σ
+def tla_not {α : Type} (p : pred α) : pred α := fun σ => ¬ p σ
+def tla_forall {α β : Type} (p : α → pred β) : pred β := fun σ => ∀ x, p x σ
+def tla_exists {α β : Type} (p : α → pred β) : pred β := fun σ => ∃ x, p x σ
 
-def action (α : Type) := α → α → Prop
-def action_pred {α : Type} (a : action α) : predicate α :=
-  λ σ ↦ a (σ 0) (σ 1)
+-- HMM how to derive all these kinds?
+instance {α : Type} : Std.Commutative (@tla_and α) := by
+  constructor ; intros ; unfold tla_and ; funext e ; ac_rfl
 
-notation:90 "⟨" p:91 "⟩" => (action_pred p)
+instance {α : Type} : Std.Associative (@tla_and α) := by
+  constructor ; intros ; unfold tla_and ; funext e ; ac_rfl
 
-def drop {α : Type} (k : ℕ) (σ : exec α) : exec α := λ n ↦ σ (n + k)
+def exec.drop {α : Type} (k : Nat) (σ : exec α) : exec α := λ n => σ (n + k)
+def always {α : Type} (p : pred α) : pred α := λ σ => ∀ k, p <| σ.drop k
+def eventually {α : Type} (p : pred α) : pred α := λ σ => ∃ k, p <| σ.drop k
+def later {α : Type} (p : pred α) : pred α := λ σ => p <| σ.drop 1
 
-notation:max σ "[" i ":]" => (drop i σ)
+theorem exec.drop_drop {α : Type} (k l : Nat) (σ : exec α) : (σ.drop k).drop l = σ.drop (k + l) := by
+  funext n ; simp [exec.drop] ; ac_rfl
 
--- @[simp]
-lemma drop_drop {α : Type} (k₀ k₁ : ℕ) (σ : exec α) : σ[k₀:][k₁:] = σ[k₀ + k₁:] :=
-  by
-    funext n
-    simp [drop]
-    apply congrArg
-    linarith
+def exec.satisfies {α : Type} (p : pred α) (σ : exec α) : Prop := p σ
+def valid {α : Type} (p : pred α) : Prop := ∀ (σ : exec α), σ.satisfies p
+def pred_implies {α : Type} (p q : pred α) : Prop := ∀ (σ : exec α), σ.satisfies p → σ.satisfies q
 
-def tla_and {α : Type} (p q : predicate α) : predicate α := λ σ ↦ p σ ∧ q σ
-def tla_or {α : Type} (p q : predicate α) : predicate α := λ σ ↦ p σ ∨ q σ
-def tla_implies {α : Type} (p q : predicate α) : predicate α := λ σ ↦ p σ → q σ
-def tla_not {α : Type} (p : predicate α) : predicate α := λ σ ↦ ¬ p σ
-def tla_forall {α β : Type} (p : α → predicate β) : predicate β := λ σ ↦ ∀ x, p x σ
-def tla_exist {α β : Type} (p : α → predicate β) : predicate β := λ σ ↦ ∃ x, p x σ
-
-infixr:55 "∧" => tla_and
-infixr:55 "∨" => tla_or
-infixr:30 "→" => tla_implies
-prefix:66 "¬" => tla_not
-notation:50 "∀" x:51 "," p:51 => (tla_forall (λ x ↦ p))
-notation:50 "∃" x:51 "," p:51 => (tla_exist (λ x ↦ p))
-
-def always {α : Type} (p : predicate α) : predicate α := λ σ ↦ ∀ k, p σ[k:]
-def eventually {α : Type} (p : predicate α) : predicate α := λ σ ↦ ∃ k, p σ[k:]
-def later {α : Type} (p : predicate α) : predicate α := λ σ ↦ p σ[1:]
-
-prefix:66 "□" => always
-prefix:66 "◇" => eventually
-prefix:66 "◯" => later
-
--- FIXME: make this an infix?
-def satisfies {α : Type} (p : predicate α) (σ : exec α) : Prop := p σ
-
-notation:55 σ:56 "⊨" p:56 => (satisfies p σ)
-
-def valid {α : Type} (p : predicate α) : Prop := ∀ σ, σ ⊨ p
-def pred_implies {α : Type} (p q : predicate α) : Prop := ∀ σ, σ ⊨ p → σ ⊨ q
-
-prefix:51 "⊢" => valid
-infix:51 "⊢" => pred_implies
+theorem pred_implies_trans {p q r : pred α} : pred_implies p q → pred_implies q r → pred_implies p r := by
+  intros h1 h2 e hp ; apply h2 ; apply h1 ; assumption
 
 def enabled {α : Type} (a : action α) (s : α) : Prop := ∃ s', a s s'
-def tla_enabled {α : Type} (a : action α) : predicate α := state_pred (enabled a)
+def tla_enabled {α : Type} (a : action α) : pred α := state_pred (enabled a)
 
-def weak_fairness {α : Type} (a : action α) : predicate α := □ (□ (tla_enabled a) → ◇⟨a⟩)
-def strong_fairness {α : Type} (a : action α) : predicate α := □ (□◇ (tla_enabled a) → ◇⟨a⟩)
+end TLA
 
-prefix:51 "𝒲ℱ" => weak_fairness
-prefix:51 "𝒮ℱ" => strong_fairness
+declare_syntax_cat tlafml
+syntax (priority := low) term:max : tlafml
+syntax "(" tlafml ")" : tlafml
+syntax "⌜ " term " ⌝" : tlafml
+syntax "⌞ " term " ⌟" : tlafml
+syntax "⟨ " term " ⟩" : tlafml
+syntax "⊤" : tlafml
+syntax "⊥" : tlafml
+syntax:max "¬" tlafml:40 : tlafml
+syntax:max "Enabled" term:40 : tlafml
+syntax:max "□" tlafml:40 : tlafml
+syntax:max "◇" tlafml:40 : tlafml
+syntax:max "◯" tlafml:40 : tlafml
+-- HMM why `syntax:arg ... ...:max` does not work, when we need multiple layers like `□ ◇ p`?
+syntax:15 tlafml:16 " → " tlafml:15 : tlafml
+syntax:35 tlafml:36 " ∧ " tlafml:35 : tlafml
+syntax:30 tlafml:31 " ∨ " tlafml:30 : tlafml
+syntax:20 tlafml:21 " ↝ " tlafml:20 : tlafml
+syntax:arg "𝒲ℱ" term:max : tlafml
 
-def leads_to {α : Type} (p q : predicate α) : predicate α := □ (p → ◇ q)
+-- the way how binders are defined and how they are expanded is taken from `Mathlib.Order.SetNotation`
+open Batteries.ExtendedBinder in
+syntax "∀ " extBinder ", " tlafml:51 : tlafml
+open Batteries.ExtendedBinder in
+syntax "∃ " extBinder ", " tlafml:51 : tlafml
 
-infix:60 "↝" => leads_to
+syntax "⋀ " binderIdent " ∈ " term ", " tlafml : tlafml
 
--- TODO until related?
+syntax "[tlafml|" tlafml "]" : term
+
+macro_rules
+  | `([tlafml| ( $f:tlafml ) ]) => `([tlafml| $f ])
+  | `([tlafml| ⌜ $t:term ⌝ ]) => `(TLA.state_pred $t)
+  | `([tlafml| ⌞ $t:term ⌟ ]) => `(TLA.pure_pred $t)
+  | `([tlafml| ⟨ $t:term ⟩ ]) => `(TLA.action_pred $t)
+  | `([tlafml| ⊤ ]) => `(TLA.tla_true)
+  | `([tlafml| ⊥ ]) => `(TLA.tla_false)
+  | `([tlafml| ¬ $f:tlafml ]) => `(TLA.tla_not [tlafml| $f ])
+  | `([tlafml| Enabled $t:term ]) => `(TLA.tla_enabled $t)
+  | `([tlafml| □ $f:tlafml ]) => `(TLA.always [tlafml| $f ])
+  | `([tlafml| ◇ $f:tlafml ]) => `(TLA.eventually [tlafml| $f ])
+  | `([tlafml| ◯ $f:tlafml ]) => `(TLA.later [tlafml| $f ])
+  | `([tlafml| $f1:tlafml → $f2:tlafml ]) => `(TLA.tla_implies [tlafml| $f1 ] [tlafml| $f2 ])
+  | `([tlafml| $f1:tlafml ∧ $f2:tlafml ]) => `(TLA.tla_and [tlafml| $f1 ] [tlafml| $f2 ])
+  | `([tlafml| $f1:tlafml ∨ $f2:tlafml ]) => `(TLA.tla_or [tlafml| $f1 ] [tlafml| $f2 ])
+  | `([tlafml| ∀ $x:ident, $f:tlafml]) => `(TLA.tla_forall fun $x:ident => [tlafml| $f ])
+  | `([tlafml| ∀ $x:ident : $t, $f:tlafml]) => `(TLA.tla_forall fun $x:ident : $t => [tlafml| $f ])
+  | `([tlafml| ∃ $x:ident, $f:tlafml]) => `(TLA.tla_exists fun $x:ident => [tlafml| $f ])
+  | `([tlafml| ∃ $x:ident : $t, $f:tlafml]) => `(TLA.tla_exists fun $x:ident : $t => [tlafml| $f ])
+  | `([tlafml| ⋀ $x:ident ∈ $l:term, $f:tlafml]) => `(List.foldr (fun $x => TLA.tla_and ([tlafml| $f ])) TLA.tla_true $l)
+  | `([tlafml| ⋀ _ ∈ $l:term, $f:tlafml]) => `(List.foldr (fun _ => TLA.tla_and ([tlafml| $f ])) TLA.tla_true $l)
+  | `([tlafml| $t:term ]) => `($t)
+
+-- these definitions are not necessarily required, but for delaboration purposes
+def TLA.leads_to {α : Type} (p q : TLA.pred α) : TLA.pred α := [tlafml| □ (p → ◇ q) ]
+def TLA.weak_fairness {α : Type} (a : action α) : pred α := [tlafml| □ ((□ (Enabled a)) → ◇ ⟨a⟩)]
+
+macro_rules
+  | `([tlafml| $f1:tlafml ↝ $f2:tlafml ]) => `(TLA.leads_to [tlafml| $f1 ] [tlafml| $f2 ])
+  | `([tlafml| 𝒲ℱ $t:term ]) => `(TLA.weak_fairness $t)
+
+-- FIXME: use something fancier like `ᴛʟᴀ`
+syntax:max tlafml:max " |-tla- " tlafml:max : term
+syntax:max "|-tla- " tlafml:max : term
+syntax:max tlafml:max " =tla= " tlafml:max : term
+syntax term " |=tla= " tlafml : term
+
+macro_rules
+  | `($f1:tlafml |-tla- $f2:tlafml) => `(TLA.pred_implies [tlafml| $f1 ] [tlafml| $f2 ])
+  | `(|-tla- $f1:tlafml) => `(TLA.valid [tlafml| $f1 ])
+  | `($f1:tlafml =tla= $f2:tlafml) => `([tlafml| $f1 ] = [tlafml| $f2 ])
+  | `($e:term |=tla= $f:tlafml) => `(TLA.exec.satisfies [tlafml| $f ] $e)
+
+-- doing a trick here, since it seems that `app_unexpander` cannot detect the case where a term is directly used as `tlafml`
+-- e.g., try removing the second branch and `#check forall (p : TLA.pred Prop), (p) |-tla- (p)`
+def TLA.tlafml_syntax_coe (stx : TSyntax `term) : Lean.PrettyPrinter.UnexpandM (TSyntax `tlafml) := do
+  match stx with
+  | `([tlafml| $f:tlafml ]) => pure f
+  | `(term|$t:term) => `(tlafml| $t:term )
+
+-- FIXME: it would be desirable to derive the things below automatically
+@[app_unexpander TLA.pure_pred] def TLA.unexpand_pure_pred : Lean.PrettyPrinter.Unexpander
+  | `($_ $p) => `([tlafml| ⌞ $p ⌟ ])
+  | _ => throw ()
+
+@[app_unexpander TLA.state_pred] def TLA.unexpand_state_pred : Lean.PrettyPrinter.Unexpander
+  | `($_ $p) => `([tlafml| ⌜ $p ⌝ ])
+  | _ => throw ()
+
+@[app_unexpander TLA.action_pred] def TLA.unexpand_action_pred : Lean.PrettyPrinter.Unexpander
+  | `($_ $p) => `([tlafml| ⟨ $p ⟩ ])
+  | _ => throw ()
+
+@[app_unexpander TLA.tla_enabled] def TLA.unexpand_tla_enabled : Lean.PrettyPrinter.Unexpander
+  | `($_ $p) => `([tlafml| Enabled $p ])
+  | _ => throw ()
+
+@[app_unexpander TLA.tla_true] def TLA.unexpand_tla_true : Lean.PrettyPrinter.Unexpander
+  | `($_) => `([tlafml| ⊤ ])
+
+@[app_unexpander TLA.tla_false] def TLA.unexpand_tla_false : Lean.PrettyPrinter.Unexpander
+  | `($_) => `([tlafml| ⊥ ])
+
+@[app_unexpander TLA.tla_and] def TLA.unexpand_tla_and : Lean.PrettyPrinter.Unexpander
+  | `($_ $stx1 $stx2) => do `([tlafml| $(← TLA.tlafml_syntax_coe stx1) ∧ $(← TLA.tlafml_syntax_coe stx2)])
+  | _ => throw ()
+
+@[app_unexpander TLA.tla_or] def TLA.unexpand_tla_or : Lean.PrettyPrinter.Unexpander
+  | `($_ $stx1 $stx2) => do `([tlafml| $(← TLA.tlafml_syntax_coe stx1) ∨ $(← TLA.tlafml_syntax_coe stx2)])
+  | _ => throw ()
+
+@[app_unexpander TLA.tla_implies] def TLA.unexpand_tla_implies : Lean.PrettyPrinter.Unexpander
+  | `($_ $stx1 $stx2) => do `([tlafml| $(← TLA.tlafml_syntax_coe stx1) → $(← TLA.tlafml_syntax_coe stx2)])
+  | _ => throw ()
+
+@[app_unexpander TLA.tla_not] def TLA.unexpand_tla_not : Lean.PrettyPrinter.Unexpander
+  | `($_ $stx) => do `([tlafml| ¬ $(← TLA.tlafml_syntax_coe stx) ])
+  | _ => throw ()
+
+@[app_unexpander TLA.always] def TLA.unexpand_always : Lean.PrettyPrinter.Unexpander
+  | `($_ $stx) => do `([tlafml| □ $(← TLA.tlafml_syntax_coe stx) ])
+  | _ => throw ()
+
+@[app_unexpander TLA.eventually] def TLA.unexpand_eventually : Lean.PrettyPrinter.Unexpander
+  | `($_ $stx) => do `([tlafml| ◇ $(← TLA.tlafml_syntax_coe stx) ])
+  | _ => throw ()
+
+@[app_unexpander TLA.later] def TLA.unexpand_later : Lean.PrettyPrinter.Unexpander
+  | `($_ $stx) => do `([tlafml| ◯ $(← TLA.tlafml_syntax_coe stx) ])
+  | _ => throw ()
+
+@[app_unexpander TLA.leads_to] def TLA.unexpand_leads_to : Lean.PrettyPrinter.Unexpander
+  | `($_ $stx1 $stx2) => do `([tlafml| $(← TLA.tlafml_syntax_coe stx1) ↝ $(← TLA.tlafml_syntax_coe stx2)])
+  | _ => throw ()
+
+@[app_unexpander TLA.weak_fairness] def TLA.unexpand_weak_fairness : Lean.PrettyPrinter.Unexpander
+  | `($_ $p) => `([tlafml| 𝒲ℱ $p ])
+  | _ => throw ()
+
+@[app_unexpander TLA.tla_forall] def TLA.unexpand_tla_forall : Lean.PrettyPrinter.Unexpander
+  | `($_ fun $a:ident => $stx)
+  | `($_ fun ($a:ident : $_) => $stx) => do `([tlafml| ∀ $a:ident, ($(← TLA.tlafml_syntax_coe stx)) ])
+  | _ => throw ()
+
+@[app_unexpander TLA.tla_exists] def TLA.unexpand_tla_exists : Lean.PrettyPrinter.Unexpander
+  | `($_ fun $a:ident => $stx)
+  | `($_ fun ($a:ident : $_) => $stx) => do `([tlafml| ∃ $a:ident, ($(← TLA.tlafml_syntax_coe stx)) ])
+  | _ => throw ()
+
+@[app_unexpander TLA.pred_implies] def TLA.unexpand_pred_implies : Lean.PrettyPrinter.Unexpander
+  | `($_ $stx1 $stx2) => do `(($(← TLA.tlafml_syntax_coe stx1)) |-tla- ($(← TLA.tlafml_syntax_coe stx2)))
+  | _ => throw ()
+
+@[app_unexpander TLA.valid] def TLA.unexpand_valid : Lean.PrettyPrinter.Unexpander
+  | `($_ $stx) => do `(|-tla- ($(← TLA.tlafml_syntax_coe stx)))
+  | _ => throw ()
+
+@[app_unexpander TLA.exec.satisfies] def TLA.unexpand_satisfies : Lean.PrettyPrinter.Unexpander
+  | `($_ $stx1 $stx2) => do `($stx2 |=tla= $(← TLA.tlafml_syntax_coe stx1))
+  | _ => throw ()
+
+@[app_unexpander Eq] def TLA.unexpand_tla_eq : Lean.PrettyPrinter.Unexpander
+  | `($_ [tlafml| $f1:tlafml ] [tlafml| $f2:tlafml ]) => `(($f1) =tla= ($f2))
+  | `($_ [tlafml| $f1:tlafml ] $t2:term) => do `(($f1) =tla= ($(← `(tlafml| $t2:term ))))
+  | `($_ $t1:term [tlafml| $f2:tlafml ]) => do `(($(← `(tlafml| $t1:term ))) =tla= ($f2))
+  | _ => throw ()
+
+@[app_unexpander List.foldr] def TLA.unexpand_tla_and_bigwedge : Lean.PrettyPrinter.Unexpander
+  | `($_ $stx1 [tlafml| ⊤ ] $l:term) =>
+    -- HMM directly writing `$stx1` as `(fun ...)` above does not work?
+    match stx1 with
+    | `(fun $x:ident => $stx)
+    | `(fun ($x:ident : $_) => $stx) =>
+      match stx with
+      | `(TLA.tla_and $stx') => do `([tlafml| ⋀ $x:ident ∈ $l:term, $(← TLA.tlafml_syntax_coe stx')])
+      | _ => throw ()
+    | _ => throw ()
+  | _ => throw ()
+
+register_simp_attr tlasimp_def
+register_simp_attr tlasimp
+register_simp_attr tladual      -- experimental
